

解

$$\begin{aligned}
 \int_0^{\frac{\pi}{4}} \sqrt{\tan x} dx &= \int_0^{\frac{\pi}{4}} \tan^{\frac{1}{2}} x dx \\
 &= \frac{\pi}{4 \cos\left(\frac{1}{2} \cdot \frac{\pi}{2}\right)} - \frac{1}{2} \sum_{k=1}^2 \cos\left[(2+1) \cdot \frac{2k-1}{2 \cdot 2} \pi\right] \log\left(2\left(1 - \cos \frac{2k-1}{2 \cdot 2} \pi\right)\right) \\
 &= \frac{\pi}{2\sqrt{2}} - \frac{1}{2} \left(\cos \frac{3}{4} \pi \log(2 - \sqrt{2}) + \cos \frac{9}{4} \pi \log(2 + \sqrt{2})\right) \\
 &= \frac{\sqrt{2}}{4} \pi - \frac{\sqrt{2}}{4} \log(1 + \sqrt{2})^2 \\
 &= \frac{\sqrt{2}}{4} \pi - \frac{\sqrt{2}}{2} \log(1 + \sqrt{2}) \cdots \cdots (\text{答})
 \end{aligned}$$

例題

次の積分を求めよ。

$$\int_0^{\frac{\pi}{4}} \tan^{\frac{3}{2}} \theta d\theta$$

解法；偶数に寄せて次数を減らす！

$$\begin{aligned}
 &\int_0^{\frac{\pi}{4}} \tan^{\frac{3}{2}} \theta d\theta \\
 &= \int_0^{\frac{\pi}{4}} (1 + \tan^2 \theta) \tan^{-\frac{1}{2}} \theta - \tan^{-\frac{1}{2}} \theta d\theta \\
 &= \left[2 \tan^{\frac{1}{2}} \theta\right]_0^{\frac{\pi}{4}} - \int_0^{\frac{\pi}{4}} \tan^{-\frac{1}{2}} \theta d\theta \\
 &= 2 - \frac{\pi}{2\sqrt{2}} + \frac{1}{2} \sum_{k=1}^2 \cos\left[(2-1) \frac{2k-1}{2 \cdot 2} \pi\right] \log\left[2\left(1 - \cos \frac{2k-1}{2 \cdot 2} \pi\right)\right] \\
 &= 2 - \frac{\sqrt{2}}{4} \pi + \frac{1}{2} \left(\cos \frac{\pi}{4} \log\left[2\left(1 - \frac{1}{\sqrt{2}}\right)\right] + \cos \frac{3}{4} \pi \log\left[2\left(1 + \frac{1}{\sqrt{2}}\right)\right]\right) \\
 &= 2 - \frac{\sqrt{2}}{4} \pi + \frac{1}{2} \left\{\frac{1}{\sqrt{2}} \log(2 - \sqrt{2}) - \frac{1}{\sqrt{2}} \log(2 + \sqrt{2})\right\} \\
 &= 2 - \frac{\sqrt{2}}{4} \pi - \frac{\sqrt{2}}{4} \log\left|\frac{\sqrt{2}+1}{\sqrt{2}-1}\right| \\
 &= 2 - \frac{\sqrt{2}}{4} \pi - \frac{\sqrt{2}}{2} \log(1 + \sqrt{2}) \cdots \cdots (\text{答})
 \end{aligned}$$